src/Refinement.v
@@ -32,10 +32,8 @@ Section refinement.
   (* 1.8 *)
   Lemma r_absorb_assumption pre' w pre post `{!FormulaFinal pre'} `{!FormulaFinal pre} :
     <{ {pre'}; *w : [pre, post] }> ≡ <{ *w : [pre' ∧ pre, post] }>.
-  Proof.
-    split; intros A; simpl.
-    - fSimpl. rewrite subst_initials_nil. rewrite f_and_assoc. reflexivity.
-    - fSimpl. rewrite subst_initials_nil. rewrite f_and_assoc. reflexivity.
+  Proof with auto.
+    intros A. simpl. repeat rewrite subst_initials_nil. fSimpl. rewrite f_and_assoc...
   Qed.
 
   (* Law 1.1 *)
@@ -73,15 +71,8 @@ Section refinement.
     w ≡ₚ w' →
     <{ *w : [pre, post] }> ≡ <{ *w' : [pre, post] }>.
   Proof with auto.
-    intros. split; intros A.
-    - simpl. fSimpl. rewrite subst_initials_perm with (xs':=w')... f_equiv.
-      rewrite f_foralllist_permute with (xs':=(fmap as_var w')).
-      + reflexivity.
-      + apply Permutation_map...
-    - symmetry in H. simpl. fSimpl. rewrite subst_initials_perm with (xs':=w)... f_equiv.
-      rewrite f_foralllist_permute with (xs':=(fmap as_var w)).
-      + reflexivity.
-      + apply Permutation_map...
+    intros H A. simpl. fSimpl. rewrite subst_initials_perm with (xs':=w')... f_equiv.
+      rewrite f_foralllist_permute with (xs':=(fmap as_var w'))... apply Permutation_map...
   Qed.
 
   (* Law 5.4 *)
@@ -330,6 +321,1142 @@ Section refinement.
     apply msubst_formula_final.
     Unshelve. typeclasses eauto.
   Qed.
+
+  (* TODO: move it *)
+  Lemma fequiv_congr A B :
+    A ≡ B → A ⇛ B.
+  Proof. intros. rewrite H. reflexivity. Qed.
+
+  Lemma rewrite_of_same_length {A B C : Type} (xs xs' : list A) (ys ys' : list B)
+      (f : ∀ (xs : list A) (ys : list B), OfSameLength xs ys → C)
+      `{!OfSameLength xs ys} `{!OfSameLength xs' ys'} :
+    xs = xs' →
+    ys = ys' →
+    f xs ys _ = f xs' ys' _.
+  Proof.
+    intros. subst. f_equiv. apply OfSameLength_pi.
+  Qed.
+
+  Lemma PAsgnWithOpens_app_nil_r lhs rhs `{!OfSameLength lhs rhs} {Hl} :
+    @PAsgnWithOpens M (lhs ++ []) (rhs ++ []) Hl = PAsgnWithOpens lhs rhs.
+  Proof with auto.
+    unfold PAsgnWithOpens.
+    replace (split_asgn_list (lhs ++ []) (rhs ++ [])) with (split_asgn_list lhs rhs);
+      [reflexivity|].
+    apply rewrite_of_same_length; rewrite app_nil_r; reflexivity.
+  Qed.
+
+  (* Lemma asgn_comm x r xs1 xs2 (rhs1 rhs2 : list (@asgn_rhs_term M)) *)
+  (*     `{!OfSameLength xs1 rhs1} *)
+  (*     `{!OfSameLength xs2 rhs2} : *)
+  (*   <{ *xs1 := *rhs1 }> ≡ <{ *xs2 := *rhs2}>. *)
+  (*   <{ *xs1, x, *xs2 := *rhs1, *[r], *rhs2 }> ≡ *)
+  (*   <{ x, *xs1, *xs2 := *[r], *rhs1, *rhs2 }>. *)
+  Definition is_open (r : @asgn_rhs_term M) :=
+    match r with
+    | OpenRhsTerm => true
+    | FinalRhsTerm t => false
+    end.
+  Definition is_closed (r : @asgn_rhs_term M) :=
+    match r with
+    | OpenRhsTerm => false
+    | FinalRhsTerm t => true
+    end.
+
+  (* Lemma wp_asgn_with_opens xs (rhs : list (@asgn_rhs_term M)) A {Hl} *)
+  (*                          `{!OfSameLength xs rhs} *)
+  (*   : *)
+  (*   wp (PAsgnWithOpens xs rhs) A ≡ *)
+  (*      wp (@PVarList M (omap (λ x, if is_open x.2 then Some x.1 else None) (zip xs rhs) : list final_variable) *)
+  (*                    (@PAsgn _ (omap (λ x, if is_open x.2 then Some x.1 else None) (zip xs rhs)) *)
+  (*                       (omap (λ x, if is_open x.2 then Some x.2 else None) (zip xs rhs)) Hl)) A. *)
+
+  (* Lemma asgn_comm_head x1 x2 r1 r2 xs (rhs : list (@asgn_rhs_term M)) *)
+  (*     `{!OfSameLength ([x1] ++ [x2] ++ xs) ([r1] ++ [r2] ++ rhs)} *)
+  (*     `{!OfSameLength ([x2] ++ [x1] ++ xs) ([r2] ++ [r1] ++ rhs)} : *)
+  (*   x1 ≠ x2 → *)
+  (*   <{ x1, x2, *xs := *$([r1]), *$([r2]), *rhs }> ≡ *)
+  (*   <{ x2, x1, *xs := *$([r2]), *$([r1]), *rhs }>. *)
+  (* Proof with auto. *)
+  (*   intros. unfold PAsgnWithOpens. unfold split_asgn_list. *)
+  (*   assert (OfSameLength xs rhs). *)
+  (*   { do 2 apply of_same_length_rest in OfSameLength0... } *)
+  (*   intros Hneq A. simpl. destruct r1, r2.  *)
+  (*   - repeat erewrite PAsgnWithOpens_cons_open. simpl. rewrite f_forall_comm... *)
+  (*   - repeat erewrite PAsgnWithOpens_cons_open. simpl. *)
+  (*     unfold PAsgnWithOpens. *)
+  (*     erewrite split_asgn_list_cons_closed. erewrite split_asgn_list_cons_closed. *)
+  (*     erewrite split_asgn_list_cons_open. *)
+  (*     unfold asgn_args_with_closed. unfold asgn_args_with_open. *)
+  (*     destruct (split_asgn_list xs rhs) eqn:E. *)
+  (*     simpl. repeat f_equiv. *)
+  (*   - repeat erewrite PAsgnWithOpens_cons_open. simpl. *)
+  (*     unfold PAsgnWithOpens. *)
+  (*     erewrite split_asgn_list_cons_closed. erewrite split_asgn_list_cons_closed. *)
+  (*     erewrite split_asgn_list_cons_open. *)
+  (*     unfold asgn_args_with_closed. unfold asgn_args_with_open. *)
+  (*     destruct (split_asgn_list xs rhs) eqn:E. *)
+  (*     simpl. repeat f_equiv. *)
+  (*   - simpl. unfold PAsgnWithOpens. *)
+  (*     erewrite split_asgn_list_cons_closed. erewrite split_asgn_list_cons_closed. *)
+  (*     erewrite split_asgn_list_cons_closed. erewrite split_asgn_list_cons_closed. *)
+  (*     unfold asgn_args_with_closed. *)
+  (*     destruct (split_asgn_list xs rhs) eqn:E. *)
+  (*     simpl. clear E. induction asgn_opens; simpl; [| rewrite IHasgn_opens; auto]. *)
+  (*     erewrite (rewrite_of_same_length *)
+  (*                 _ ([] ++ [as_var x1] ++ [as_var x2] *)
+  (*                      ++ (list_fmap final_variable variable as_var asgn_xs)) *)
+  (*                 _ ([] ++ [as_term t] ++ [as_term t0] *)
+  (*                      ++ list_fmap final_term term as_term asgn_ts))... *)
+  (*     rewrite (msubst_comm_consecutive A [] [] (as_var x1) (as_term t) (as_var x2) (as_term t0))... *)
+  (*     1-2: typeclasses eauto. *)
+  (*     intros contra. apply as_var_inj in contra. subst. done. *)
+  (* Qed. *)
+  (* Lemma asgn_comm_tail x1 x2 r1 r2 xs (rhs : list (@asgn_rhs_term M)) *)
+  (*     `{!OfSameLength (xs ++ [x1] ++ [x2]) (rhs ++ [r1] ++ [r2])} *)
+  (*     `{!OfSameLength (xs ++ [x2] ++ [x1]) (rhs ++ [r2] ++ [r1])} : *)
+  (*   x1 ≠ x2 → *)
+  (*   <{ *xs, x1, x2 := *rhs, *$([r1]), *$([r2]) }> ≡ *)
+  (*   <{ *xs, x2, x1 := *rhs, *$([r2]), *$([r1]) }>. *)
+  (* Proof with auto. *)
+  (*   assert (OfSameLength xs rhs). *)
+  (*   {unfold OfSameLength in *. repeat rewrite length_app in OfSameLength0. *)
+  (*     simpl in OfSameLength0. lia. } *)
+  (*   intros Hneq A. simpl. *)
+  (*   induction_same_length xs rhs as x' r'. *)
+  (*   - simpl. apply asgn_comm_head... *)
+  (*   - intros. simpl. destruct r'. *)
+  (*   destruct r1, r2.  *)
+  (*   - repeat erewrite PAsgnWithOpens_cons_open. simpl. rewrite f_forall_comm... *)
+  (*   - repeat erewrite PAsgnWithOpens_cons_open. simpl. *)
+  (*     unfold PAsgnWithOpens. *)
+  (*     erewrite split_asgn_list_cons_closed. erewrite split_asgn_list_cons_closed. *)
+  (*     erewrite split_asgn_list_cons_open. *)
+  (*     unfold asgn_args_with_closed. unfold asgn_args_with_open. *)
+  (*     destruct (split_asgn_list xs rhs) eqn:E. *)
+  (*     simpl. repeat f_equiv. *)
+  (*   - repeat erewrite PAsgnWithOpens_cons_open. simpl. *)
+  (*     unfold PAsgnWithOpens. *)
+  (*     erewrite split_asgn_list_cons_closed. erewrite split_asgn_list_cons_closed. *)
+  (*     erewrite split_asgn_list_cons_open. *)
+  (*     unfold asgn_args_with_closed. unfold asgn_args_with_open. *)
+  (*     destruct (split_asgn_list xs rhs) eqn:E. *)
+  (*     simpl. repeat f_equiv. *)
+  (*   - simpl. unfold PAsgnWithOpens. *)
+  (*     erewrite split_asgn_list_cons_closed. erewrite split_asgn_list_cons_closed. *)
+  (*     erewrite split_asgn_list_cons_closed. erewrite split_asgn_list_cons_closed. *)
+  (*     unfold asgn_args_with_closed. *)
+  (*     destruct (split_asgn_list xs rhs) eqn:E. *)
+  (*     simpl. clear E. induction asgn_opens; simpl; [| rewrite IHasgn_opens; auto]. *)
+  (*     erewrite (rewrite_of_same_length *)
+  (*                 _ ([] ++ [as_var x1] ++ [as_var x2] *)
+  (*                      ++ (list_fmap final_variable variable as_var asgn_xs)) *)
+  (*                 _ ([] ++ [as_term t] ++ [as_term t0] *)
+  (*                      ++ list_fmap final_term term as_term asgn_ts))... *)
+  (*     rewrite (msubst_comm_consecutive A [] [] (as_var x1) (as_term t) (as_var x2) (as_term t0))... *)
+  (*     1-2: typeclasses eauto. *)
+  (*     intros contra. apply as_var_inj in contra. subst. done. *)
+  (* Qed. *)
+  Global Instance PVar_proper : Proper ((=) ==> (≡) ==> (≡@{prog})) PVar.
+  Proof. intros x ? <- A B ? C. simpl. rewrite (H C). reflexivity. Qed.
+
+  Global Instance PVarList_proper : Proper ((=) ==> (≡) ==> (≡@{prog})) PVarList.
+  Proof.
+    intros xs ? <- A B ? C. induction xs as [|x xs IH].
+    - simpl. apply H.
+    - simpl. rewrite IH. reflexivity.
+  Qed.
+
+  Lemma wp_varlist xs p A :
+    wp (PVarList xs p) A ≡ <! ∀* ↑ₓ xs, $(wp p A) !>.
+  Proof with auto. induction xs as [|x xs IH]... simpl. rewrite IH. reflexivity. Qed.
+
+  Lemma p_varlist_permute xs xs' (p : prog) :
+    xs ≡ₚ xs' →
+    PVarList xs p ≡ PVarList xs' p.
+  Proof.
+    intros Hperm A. do 2 rewrite wp_varlist. rewrite f_foralllist_permute; [reflexivity|].
+    apply Permutation_map. assumption.
+  Qed.
+
+  Lemma p_varlist_app xs1 xs2 (p : prog) :
+    PVarList (xs1 ++ xs2) p ≡ PVarList (xs2 ++ xs1) p.
+  Proof with auto.
+    intros A. do 2 rewrite wp_varlist. do 2 rewrite fmap_app.
+    do 2 rewrite foralllist_app. rewrite f_foralllist_comm...
+  Qed.
+
+Lemma elem_of_zip_pair_nil {A B : Type} x y :
+  (x, y) ∈ (([] : list A), ([] : list B)) → False.
+Proof with auto.
+  intros (i&?&?). simpl in *. apply elem_of_list_lookup_2 in H. set_solver.
+Qed.
+
+Lemma elem_of_zip_pair_hd_ne {A B : Type} x0 y0 x y (xs : list A) (ys : list B) :
+  x0 ≠ x →
+  (x0, y0) ∈ (x :: xs, y :: ys) ↔ (x0, y0) ∈ (xs, ys).
+Proof with auto.
+  intros. split; intros (i&?).
+  - destruct i.
+    + apply elem_of_zip_pair_hd_indexed in H0 as []. subst. contradiction.
+    + apply elem_of_zip_pair_tl_indexed in H0. exists i...
+  - exists (S i). apply elem_of_zip_pair_tl_indexed...
+Qed.
+
+Lemma elem_of_zip_pair_hd {A B : Type} y0 x y (xs : list A) (ys : list B) :
+  x ∉ xs →
+  (x, y0) ∈ (x :: xs, y :: ys) ↔ y0 = y.
+Proof with auto.
+  intros. split.
+  - intros (i&?). destruct i.
+    + apply elem_of_zip_pair_hd_indexed in H0 as []...
+    + apply elem_of_zip_pair_tl_indexed in H0 as []. simpl in *. apply elem_of_list_lookup_2 in H0.
+      done.
+  - intros ->. exists 0. apply elem_of_zip_pair_hd_indexed...
+Qed.
+
+Lemma elem_of_zip_pair_app {A B : Type} x y (xs1 : list A) (ys1 : list B)
+  (xs2 : list A) (ys2 : list B) `{!OfSameLength xs1 ys1} :
+  (x, y) ∈ (xs1 ++ xs2, ys1 ++ ys2) ↔ (x, y) ∈ (xs1, ys1) ∨ (x, y) ∈ (xs2, ys2).
+Proof with auto.
+  split.
+  - intros (i&?&?). simpl in H, H0. destruct (decide (i < length xs1)).
+    + left. rewrite lookup_app_l in H... rewrite OfSameLength0 in l. rewrite lookup_app_l in H0...
+      exists i. split...
+    + right. rewrite lookup_app_r in H by lia. rewrite OfSameLength0 in n.
+      rewrite lookup_app_r in H0 by lia. rewrite OfSameLength0 in H. exists (i - length ys1).
+      split...
+  - intros [|]; destruct H as (i&?&?); simpl in H, H0.
+    + exists i. split; simpl; apply lookup_app_l_Some...
+    + exists (length xs1 + i). split; simpl.
+      * rewrite lookup_app_r by lia. replace (length xs1 + i - length xs1) with i by lia...
+      * rewrite OfSameLength0. rewrite lookup_app_r by lia.
+        replace (length ys1 + i - length ys1) with i by lia...
+Qed.
+
+Lemma elem_of_zip_pair_indexed_inv {A B : Type} i x y (xs : list A) (ys : list B) :
+  (i, (x, y)) ∈ (xs, ys) → (x, y) ∈ (xs, ys).
+Proof. intros. exists i. assumption. Qed.
+
+Lemma asgn_opens_with_open x lhs rhs `{!OfSameLength lhs rhs} :
+  asgn_opens (asgn_args_with_open (split_asgn_list lhs rhs) x) =
+    x :: @asgn_opens M (split_asgn_list lhs rhs).
+Proof.
+  destruct (split_asgn_list lhs rhs). simpl. reflexivity.
+Qed.
+
+Lemma asgn_opens_with_closed x t lhs rhs `{!OfSameLength lhs rhs} :
+  asgn_opens (asgn_args_with_closed (split_asgn_list lhs rhs) x t) =
+    @asgn_opens M (split_asgn_list lhs rhs).
+Proof.
+  destruct (split_asgn_list lhs rhs). simpl. reflexivity.
+Qed.
+
+Lemma asgn_xs_with_open x lhs rhs `{!OfSameLength lhs rhs} :
+  asgn_xs (asgn_args_with_open (split_asgn_list lhs rhs) x) =
+    @asgn_xs M (split_asgn_list lhs rhs).
+Proof.
+  destruct (split_asgn_list lhs rhs). simpl. reflexivity.
+Qed.
+
+Lemma asgn_xs_with_closed x t lhs rhs `{!OfSameLength lhs rhs} :
+  asgn_xs (asgn_args_with_closed (split_asgn_list lhs rhs) x t) =
+    x :: @asgn_xs M (split_asgn_list lhs rhs).
+Proof.
+  destruct (split_asgn_list lhs rhs). simpl. reflexivity.
+Qed.
+
+Lemma asgn_ts_with_open x lhs rhs `{!OfSameLength lhs rhs} :
+  asgn_ts (asgn_args_with_open (split_asgn_list lhs rhs) x) =
+    @asgn_ts M (split_asgn_list lhs rhs).
+Proof.
+  destruct (split_asgn_list lhs rhs). simpl. reflexivity.
+Qed.
+
+Lemma asgn_ts_with_closed x t lhs rhs `{!OfSameLength lhs rhs} :
+  asgn_ts (asgn_args_with_closed (split_asgn_list lhs rhs) x t) =
+    t :: @asgn_ts M (split_asgn_list lhs rhs).
+Proof.
+  destruct (split_asgn_list lhs rhs). simpl. reflexivity.
+Qed.
+
+Lemma elem_of_asgn_opens x lhs rhs `{!OfSameLength lhs rhs} :
+  NoDup lhs →
+  x ∈ asgn_opens (split_asgn_list lhs rhs) ↔ (x, @OpenRhsTerm M) ∈ (lhs, rhs).
+Proof with auto.
+  induction_same_length lhs rhs as l r.
+  - simpl. unfold zip_pair_elem_of. pose proof (elem_of_zip_pair_nil x (@OpenRhsTerm M)).
+    set_solver.
+  - intros. assert (Hl := of_same_length_rest H'). apply NoDup_cons in H as [].
+    destruct (decide (x = l)).
+    2:{ rewrite elem_of_zip_pair_hd_ne... destruct r.
+        - erewrite split_asgn_list_cons_open. rewrite asgn_opens_with_open.
+          rewrite elem_of_cons. rewrite IH... naive_solver.
+        - erewrite split_asgn_list_cons_closed. rewrite asgn_opens_with_closed.
+          rewrite IH... }
+    subst l. destruct r.
+    + erewrite split_asgn_list_cons_open. rewrite asgn_opens_with_open.
+      rewrite elem_of_cons. rewrite IH... rewrite elem_of_zip_pair_hd... split...
+    + erewrite split_asgn_list_cons_closed. rewrite asgn_opens_with_closed.
+      rewrite IH... rewrite elem_of_zip_pair_hd... split; [|discriminate]. intros (i&?&?).
+      simpl in H1, H2. apply elem_of_list_lookup_2 in H1. contradiction.
+Qed.
+
+Lemma elem_of_asgn_xs_ts x t lhs rhs `{!OfSameLength lhs rhs} :
+  NoDup lhs →
+  (x, t) ∈ (asgn_xs (split_asgn_list lhs rhs), asgn_ts (split_asgn_list lhs rhs)) ↔
+         (x, @FinalRhsTerm M t) ∈ (lhs, rhs).
+Proof with auto.
+  induction_same_length lhs rhs as l r.
+  - simpl. unfold zip_pair_elem_of. pose proof (elem_of_zip_pair_nil x t).
+    pose proof (elem_of_zip_pair_nil x (@FinalRhsTerm M t)). set_solver.
+  - intros. assert (Hl := of_same_length_rest H'). apply NoDup_cons in H as [].
+    destruct (decide (x = l)).
+    2:{ rewrite elem_of_zip_pair_hd_ne... destruct r.
+        - erewrite split_asgn_list_cons_open. rewrite asgn_xs_with_open.
+          rewrite asgn_ts_with_open. rewrite IH...
+        - erewrite split_asgn_list_cons_closed. rewrite asgn_xs_with_closed.
+          rewrite asgn_ts_with_closed. rewrite elem_of_zip_pair_hd_ne... }
+    subst l. destruct r.
+    + erewrite split_asgn_list_cons_open. rewrite asgn_xs_with_open. rewrite asgn_ts_with_open.
+      rewrite IH... rewrite elem_of_zip_pair_hd... split; [|discriminate]. intros (i&?&?).
+      simpl in H1, H2. apply elem_of_list_lookup_2 in H1. contradiction.
+    + erewrite split_asgn_list_cons_closed. rewrite asgn_xs_with_closed.
+      rewrite asgn_ts_with_closed. rewrite (elem_of_zip_pair_hd (FinalRhsTerm t))...
+      split.
+      * intros (i&?). destruct i.
+        -- apply elem_of_zip_pair_hd_indexed in H1 as [_ ?]. subst...
+        -- apply elem_of_zip_pair_tl_indexed in H1. apply elem_of_zip_pair_indexed_inv in H1.
+           rewrite IH in H1... destruct H1 as (j&?&?). simpl in H1.
+           apply elem_of_list_lookup_2 in H1. contradiction.
+      * intros. inversion H1. subst t0. exists 0. split; simpl...
+Qed.
+
+Global Instance wp_proper_prog {A : final_formula} : Proper ((≡@{prog}) ==> (≡)) (λ p, wp p A).
+Proof. intros p1 p2 Hp. specialize (Hp A). assumption. Qed.
+
+Definition zip_pair_Permutation {A B : Type} (p1 p2 : list A * list B) :=
+  ∀ (x : A) (y : B), (x, y) ∈ p1 ↔ (x, y) ∈ p2.
+
+Infix "≡ₚₚ" := (zip_pair_Permutation) (at level 70, no associativity) : refiney_scope.
+
+Global Instance zip_pair_Permutation_refl {A B : Type} : Reflexive (@zip_pair_Permutation A B).
+Proof. intros p x y. reflexivity. Qed.
+
+Hint Extern 0 (?p ≡ₚₚ ?p) => reflexivity : core.
+
+Global Instance zip_pair_Permutation_sym {A B : Type} : Symmetric (@zip_pair_Permutation A B).
+Proof. intros p1 p2 H x y. specialize (H x y). naive_solver. Qed.
+
+Global Instance zip_pair_Permutation_trans {A B : Type} : Transitive (@zip_pair_Permutation A B).
+Proof.
+  intros p1 p2 p3 H12 H23. intros x y. specialize (H12 x y). specialize (H23 x y). naive_solver.
+Qed.
+
+Global Instance zip_pair_Permutation_equiv {A B : Type} : Equivalence (@zip_pair_Permutation A B).
+Proof.
+  split; [exact zip_pair_Permutation_refl | exact zip_pair_Permutation_sym |
+           exact zip_pair_Permutation_trans].
+Qed.
+
+Lemma zip_pair_Permutation_cons {A B : Type} `{EqDecision A} (x : A) (y : B) (xs1 : list A)
+  (ys1 : list B) (xs2 : list A) (ys2 : list B) `{!OfSameLength xs1 ys1} `{!OfSameLength xs2 ys2} :
+  (* x ∉ xs1 → *)
+  (* x ∉ xs2 → *)
+  (xs1, ys1) ≡ₚₚ (xs2, ys2) →
+  (x :: xs1, y :: ys1) ≡ₚₚ (x :: xs2, y :: ys2).
+Proof with auto.
+  unfold zip_pair_Permutation. intros. split; intros (i&?&?); simpl in H0, H1.
+  - destruct i.
+    + exists 0. split...
+    + rewrite lookup_cons_ne_0 in H0 by lia. simpl in H0.
+      rewrite lookup_cons_ne_0 in H1 by lia. simpl in H1. specialize (H x0 y0).
+      pose proof (proj1 H). forward H2 by (exists i; split; auto).
+      destruct H2 as (j&?&?). simpl in H2, H3.
+      exists (S j). split...
+  - destruct i.
+    + exists 0. split...
+    + rewrite lookup_cons_ne_0 in H0 by lia. simpl in H0.
+      rewrite lookup_cons_ne_0 in H1 by lia. simpl in H1. specialize (H x0 y0).
+      pose proof (proj2 H). forward H2 by (exists i; split; auto).
+      destruct H2 as (j&?&?). simpl in H2, H3.
+      exists (S j). split...
+Qed.
+
+Lemma zip_pair_Permutation_app_comm {A B : Type} (xs1 : list A) (ys1 : list B) (xs2 : list A)
+    (ys2 : list B) `{!OfSameLength xs1 ys1} `{!OfSameLength xs2 ys2} :
+  (xs1 ++ xs2, ys1 ++ ys2) ≡ₚₚ (xs2 ++ xs1, ys2 ++ ys1).
+Proof with auto.
+  unfold zip_pair_Permutation. intros x y. repeat rewrite elem_of_zip_pair_app...
+  naive_solver.
+Qed.
+
+(* Global Instance app_zip_pair_Permutation {A B : Type} : *)
+(*   Proper ((@zip_pair_Permutation A B) ==>  *)
+(*   (@zip_pair_Permutation A B) ==> (@zip_pair_Permutation A B)) app. *)
+
+Lemma lookup_list_to_map_zip_Some_inv {K A : Type} `{Countable K}
+    (ks : list K) (xs : list A) (k : K) (x : A) `{!OfSameLength ks xs} :
+  (list_to_map (zip ks xs) : gmap K A) !! k = Some x →
+                                                   (k, x) ∈ (ks, xs).
+Proof with auto.
+  intros. apply lookup_list_to_map_zip_Some in H0 as (i&?&?&?)... exists i. split...
+Qed.
+
+(* Lemma zip_pair_Permutation_NoDup_dom_l {A B : Type} *)
+(*                                        `{EqDecision A} *)
+(*     (xs : list A) (ys : list B) (xs' : list A) (ys' : list B)  *)
+(*     `{!OfSameLength xs ys} `{!OfSameLength xs' ys'} : *)
+(*   (xs, ys) ≡ₚₚ (xs', ys') → *)
+(*   NoDup xs → *)
+(*   NoDup xs'. *)
+(* Proof with auto. *)
+(*   intros. unfold zip_pair_Permutation in H. destruct (decide (NoDup xs'))... *)
+(*   exfalso. rewrite NoDup_alt in n. apply n. clear n. intros i j x' ??. *)
+(*   destruct (lookup_of_same_length_l ys' H1) as (y'&?).  *)
+(*   destruct (lookup_of_same_length_l ys' H2) as (y''&?).  *)
+(*   assert ((x', y') ∈ (xs', ys')). *)
+(*   { exists i. split... } *)
+(*   assert ((x', y'') ∈ (xs', ys')). *)
+(*   { exists j. split... } *)
+(*   rewrite <- H in H5. rewrite <- H in H6. destruct H5 as (k&?&?), H6 as (l&?&?). *)
+(*   simpl in *. assert (l = k) as ->. *)
+(*   { eapply NoDup_lookup; [exact H0 | exact H6 | exact H5]. } *)
+(*   rewrite H7 in H8. inversion H8. subst y''. clear dependent xs ys H8. *)
+(*   rewrite <- H3 in H4.  *)
+
+(*   Search (¬ NoDup ?A → ?P). *)
+
+(*   NoDup *)
+(*   intros x. *)
+(*   unfold elem_of, zip_pair_elem_of in H. *)
+(*   unfold elem_of, zip_pair_elem_of_with_index in H. simpl in H. *)
+(*   apply permutations_Permutation. apply permutations *)
+(*   Permutation_ *)
+(*   generalize dependent xs'. induction_same_length xs ys as x y. *)
+(*   - apply zip_pair_Permutation_nil_inv_l in H0 as [-> ->]... *)
+(*   - intros. assert (Hl:=of_same_length_rest H'). apply zip_pair_Permutation_cons_inv_l in H... *)
+(*     destruct H as (xs'0&ys'0&xs'1&ys'1&?&?&?&?). subst.  *)
+(*     apply IH. *)
+(*     `{!EqDecision A} `{!Countable A} `{!OfSameLength xs' ys'} : *)
+
+Lemma zip_pair_Permutation_nil_inv_l {A B : Type}
+    (xs : list A) (ys : list B) `{!OfSameLength xs ys} :
+  ([], []) ≡ₚₚ (xs, ys) →
+  xs = [] ∧ ys = [].
+Proof with auto.
+  intros. unfold zip_pair_Permutation in H. induction_same_length xs ys as x y...
+  - intros. clear IH. specialize (H x y). assert ((x, y) ∈ (x :: xs, y :: ys)).
+    { exists 0. split... }
+    rewrite <- H in H0. destruct H0 as (i&?&?). simpl in H0, H1. set_solver.
+Qed.
+
+Lemma zip_pair_Permutation_cons_inv_l {A B : Type} `{EqDecision A}
+  (x : A) (y : B) (xs : list A) (ys : list B)
+  (xs' : list A) (ys' : list B) `{!OfSameLength xs ys} `{!OfSameLength xs' ys'} :
+  (x :: xs, y :: ys) ≡ₚₚ (xs', ys') →
+  x ∉ xs →
+  NoDup xs →
+  NoDup xs' →
+  ∃ (xs'0 : list A) (ys'0 : list B) (xs'1 : list A) (ys'1 : list B) (Hl0 : OfSameLength xs'0 ys'0) (Hl1 : OfSameLength xs'1 ys'1),
+    xs' = xs'0 ++ x :: xs'1 ∧ ys' = ys'0 ++ y :: ys'1 ∧ (xs, ys) ≡ₚₚ (xs'0 ++ xs'1, ys'0 ++ ys'1).
+Proof with auto.
+  intros ? Hnin Hnodup Hnodup'. pose proof (H x y). assert ((x, y) ∈ (xs', ys')) as (i&?&?).
+  { apply H. exists 0. split... }
+  simpl in H1, H2. apply elem_of_list_split_length in H1, H2. destruct H1 as (xs'0&xs'1&?&?).
+  destruct H2 as (ys'0&ys'1&?&?). subst. exists xs'0, ys'0, xs'1, ys'1. eexists; [naive_solver|].
+  eexists...
+  { pose proof (@of_same_length _ _ _ _ OfSameLength1). unfold OfSameLength.
+    repeat rewrite length_app in H1. simpl in H1. lia. }
+  split_and!... intros x' y'. specialize (H x' y').
+  apply NoDup_app in Hnodup' as (?&?&?). apply NoDup_cons in H3 as [].
+  destruct (decide (x' = x)).
+  - subst. split; intros (i&?&_); simpl in H6.
+    + apply elem_of_list_lookup_2 in H6. contradiction.
+    + apply elem_of_list_lookup_2 in H6. set_solver.
+  - rewrite elem_of_zip_pair_hd_ne in H... rewrite H.
+    rewrite elem_of_zip_pair_app... rewrite elem_of_zip_pair_hd_ne...
+    rewrite elem_of_zip_pair_app...
+Qed.
+
+Lemma zip_pair_Permutation_list_to_map_zip {A B : Type}
+    (xs : list A) (ys : list B) (xs' : list A) (ys' : list B) `{Countable A} `{EqDecision A}
+    `{!OfSameLength xs ys} `{!OfSameLength xs' ys'} :
+  NoDup xs →
+  NoDup xs' →
+  (xs, ys) ≡ₚₚ (xs', ys') →
+  (list_to_map (zip xs ys) : gmap A B) = list_to_map (zip xs' ys').
+Proof with auto.
+  intros. unfold zip_pair_Permutation in H. apply map_eq. intros x.
+  destruct (list_to_map (zip xs ys) !! x) as [y|] eqn:E.
+  - apply lookup_list_to_map_zip_Some_inv in E... apply H2 in E.
+    symmetry. apply lookup_list_to_map_zip_Some... destruct E as (i&?&?). simpl in H3, H4.
+    exists i. split_and!... intros. apply NoDup_lookup with (i:=i) in H5... lia.
+  - apply lookup_list_to_map_zip_None in E... symmetry. apply lookup_list_to_map_zip_None...
+    intros ?. apply elem_of_list_lookup in H3 as (i&?).
+    destruct (lookup_of_same_length_l ys' H3) as (y&?)...
+    assert ((x, y) ∈ (xs, ys)) as (?&?&_).
+    { apply H2. exists i. split... }
+    simpl in H5. apply elem_of_list_lookup_2 in H5. contradiction.
+Qed.
+
+
+  Lemma msubst_zip_pair_Permutation A (xs : list variable) ts (xs' : list variable) ts' `{!OfSameLength xs ts} `{!OfSameLength xs' ts'} :
+    NoDup xs →
+    NoDup xs' →
+    (xs, ts) ≡ₚₚ (xs', ts') →
+    msubst A (to_var_term_map xs ts) ≡ msubst A (to_var_term_map xs' ts').
+  Proof with auto.
+    intros. f_equiv. apply zip_pair_Permutation_list_to_map_zip... typeclasses eauto.
+  Qed.
+
+  Lemma asgn_xs_submseteq lhs rhs `{!OfSameLength lhs rhs} :
+    @asgn_xs M (split_asgn_list lhs rhs) ⊆+ lhs.
+  Proof with auto.
+    induction_same_length lhs rhs as l r; [set_solver|]. apply submseteq_cons_r.
+    assert (Hl:=of_same_length_rest H'). destruct r.
+    - left. erewrite split_asgn_list_cons_open. rewrite asgn_xs_with_open. apply IH.
+    - right. erewrite split_asgn_list_cons_closed. rewrite asgn_xs_with_closed. eexists.
+      split; [reflexivity | apply IH].
+  Qed.
+
+  Lemma submseteq_NoDup {A : Type} (l k : list A) :
+    NoDup k →
+    l ⊆+ k →
+    NoDup l.
+  Proof with auto.
+    intros. apply submseteq_Permutation in H0 as [k' ?]. apply Permutation_NoDup in H0...
+    2:{ apply NoDup_ListNoDup... }
+    apply NoDup_ListNoDup in H0. apply NoDup_app in H0 as [? _]...
+  Qed.
+
+Lemma elem_of_zip_pair_fmap {A A' B B' : Type} x' y' (xs : list A) (ys : list B)
+    (f : A → A') (g : B → B')
+    `{!OfSameLength xs ys} `{!OfSameLength (f <$> xs) (g <$> ys)} :
+  (x', y') ∈ (f <$> xs, g <$> ys) ↔ ∃ x y, (x, y) ∈ (xs, ys) ∧ x' = f x ∧ y' = g y.
+Proof with auto.
+  split.
+  - intros (i&?&?). simpl in H, H0. apply list_lookup_fmap_Some in H as (x&?&?).
+    apply list_lookup_fmap_Some in H0 as (y&?&?). exists x, y. split_and!... exists i.
+    split...
+  - intros (x&y&(i&?&?)&?&?). simpl in H, H0. exists i. split; simpl; apply list_lookup_fmap_Some.
+    + exists x. split...
+    + exists y. split...
+Qed.
+
+Lemma zip_pair_Permutation_fmap {A A' B B' : Type}
+    (xs : list A) (ys : list B)
+    (xs' : list A) (ys' : list B)
+    (f : A → A') (g : B → B')
+    `{!OfSameLength xs ys} `{!OfSameLength (f <$> xs) (g <$> ys)}
+    `{!OfSameLength xs' ys'} `{!OfSameLength (f <$> xs') (g <$> ys')} :
+  (xs, ys) ≡ₚₚ (xs', ys') →
+  (f <$> xs, g <$> ys) ≡ₚₚ (f <$> xs', g <$> ys').
+Proof with auto.
+  intros. unfold zip_pair_Permutation. intros x' y'. rewrite elem_of_zip_pair_fmap...
+  rewrite elem_of_zip_pair_fmap... split; intros (x&y&?&?&?);
+    exists x, y; split; auto; apply H in H0...
+Qed.
+
+Lemma asgn_opens_app lhs1 rhs1 lhs2 rhs2
+  `{!OfSameLength lhs1 rhs1} `{!OfSameLength lhs2 rhs2}
+  `{!OfSameLength (lhs1 ++ lhs2) (rhs1 ++ rhs2)} :
+  asgn_opens (split_asgn_list (lhs1 ++ lhs2) (rhs1 ++ rhs2)) =
+    asgn_opens (split_asgn_list lhs1 rhs1) ++ @asgn_opens M (split_asgn_list lhs2 rhs2).
+Proof with auto.
+  generalize dependent rhs2. generalize dependent lhs2. induction_same_length lhs1 rhs1 as l1 r1;
+    simpl.
+  - repeat f_equiv. apply OfSameLength_pi.
+  - intros. assert (Hl1:=of_same_length_rest H'). destruct r1.
+    + erewrite split_asgn_list_cons_open. rewrite asgn_opens_with_open.
+      erewrite split_asgn_list_cons_open. rewrite asgn_opens_with_open.
+      erewrite IH. set_solver.
+    + erewrite split_asgn_list_cons_closed. rewrite asgn_opens_with_closed.
+      erewrite split_asgn_list_cons_closed. rewrite asgn_opens_with_closed.
+      erewrite IH...
+Qed.
+
+Lemma asgn_xs_app lhs1 rhs1 lhs2 rhs2
+  `{!OfSameLength lhs1 rhs1} `{!OfSameLength lhs2 rhs2}
+  `{!OfSameLength (lhs1 ++ lhs2) (rhs1 ++ rhs2)} :
+  asgn_xs (split_asgn_list (lhs1 ++ lhs2) (rhs1 ++ rhs2)) =
+    asgn_xs (split_asgn_list lhs1 rhs1) ++ @asgn_xs M (split_asgn_list lhs2 rhs2).
+Proof with auto.
+  generalize dependent rhs2. generalize dependent lhs2. induction_same_length lhs1 rhs1 as l1 r1;
+    simpl.
+  - repeat f_equiv. apply OfSameLength_pi.
+  - intros. assert (Hl1:=of_same_length_rest H'). destruct r1.
+    + erewrite split_asgn_list_cons_open. rewrite asgn_xs_with_open.
+      erewrite split_asgn_list_cons_open. rewrite asgn_xs_with_open.
+      erewrite IH. set_solver.
+    + erewrite split_asgn_list_cons_closed. rewrite asgn_xs_with_closed.
+      erewrite split_asgn_list_cons_closed. rewrite asgn_xs_with_closed.
+      erewrite IH...
+Qed.
+
+Lemma asgn_ts_app lhs1 rhs1 lhs2 rhs2
+  `{!OfSameLength lhs1 rhs1} `{!OfSameLength lhs2 rhs2}
+  `{!OfSameLength (lhs1 ++ lhs2) (rhs1 ++ rhs2)} :
+  asgn_ts (split_asgn_list (lhs1 ++ lhs2) (rhs1 ++ rhs2)) =
+    asgn_ts (split_asgn_list lhs1 rhs1) ++ @asgn_ts M (split_asgn_list lhs2 rhs2).
+Proof with auto.
+  generalize dependent rhs2. generalize dependent lhs2. induction_same_length lhs1 rhs1 as l1 r1;
+    simpl.
+  - repeat f_equiv. apply OfSameLength_pi.
+  - intros. assert (Hl1:=of_same_length_rest H'). destruct r1.
+    + erewrite split_asgn_list_cons_open. rewrite asgn_ts_with_open.
+      erewrite split_asgn_list_cons_open. rewrite asgn_ts_with_open.
+      erewrite IH. set_solver.
+    + erewrite split_asgn_list_cons_closed. rewrite asgn_ts_with_closed.
+      erewrite split_asgn_list_cons_closed. rewrite asgn_ts_with_closed.
+      erewrite IH...
+Qed.
+
+Lemma asgn_opens_Permutation lhs rhs lhs' rhs'
+  `{!OfSameLength lhs rhs} `{!OfSameLength lhs' rhs'} :
+  NoDup lhs →
+  NoDup lhs' →
+  (lhs, rhs) ≡ₚₚ (lhs', rhs') →
+  asgn_opens (split_asgn_list lhs rhs) ≡ₚ @asgn_opens M (split_asgn_list lhs' rhs').
+Proof with auto.
+  generalize dependent lhs'. generalize dependent rhs'. induction_same_length lhs rhs as l r.
+  - apply zip_pair_Permutation_nil_inv_l in H2... destruct H2 as [-> ->]. simpl...
+  - intros. apply NoDup_cons in H as []. assert (Hl:=of_same_length_rest H').
+    apply zip_pair_Permutation_cons_inv_l in H1...
+    destruct H1 as (xs'0&ys'0&xs'1&ys'1&?&?&?&?&?). destruct r.
+    + erewrite split_asgn_list_cons_open. rewrite asgn_opens_with_open.
+      subst. erewrite asgn_opens_app. erewrite split_asgn_list_cons_open.
+      rewrite asgn_opens_with_open. rewrite app_Permutation_comm.
+      simpl. f_equiv. etrans.
+      * apply IH with (lhs':=xs'0 ++ xs'1) (rhs':=ys'0 ++ ys'1)...
+        apply NoDup_app in H0 as (?&?&?). apply NoDup_cons in H3 as []. apply NoDup_app.
+        split_and!... intros. apply H1 in H6. set_solver.
+      * erewrite asgn_opens_app. apply Permutation_app_comm.
+    + erewrite split_asgn_list_cons_closed. rewrite asgn_opens_with_closed.
+      subst. erewrite asgn_opens_app. erewrite split_asgn_list_cons_closed.
+      rewrite asgn_opens_with_closed. rewrite app_Permutation_comm.
+      simpl. etrans.
+      * apply IH with (lhs':=xs'0 ++ xs'1) (rhs':=ys'0 ++ ys'1)...
+        apply NoDup_app in H0 as (?&?&?). apply NoDup_cons in H3 as []. apply NoDup_app.
+        split_and!... intros. apply H1 in H6. set_solver.
+      * erewrite asgn_opens_app. apply Permutation_app_comm.
+Qed.
+
+Lemma asgn_xs_ts_Permutation lhs rhs lhs' rhs'
+  `{!OfSameLength lhs rhs} `{!OfSameLength lhs' rhs'} :
+  NoDup lhs →
+  NoDup lhs' →
+  (lhs, rhs) ≡ₚₚ (lhs', rhs') →
+  (asgn_xs (split_asgn_list lhs rhs), asgn_ts (split_asgn_list lhs rhs)) ≡ₚₚ
+    (asgn_xs (split_asgn_list lhs' rhs'), @asgn_ts M (split_asgn_list lhs' rhs')).
+Proof with auto.
+  generalize dependent lhs'. generalize dependent rhs'. induction_same_length lhs rhs as l r.
+  - apply zip_pair_Permutation_nil_inv_l in H2... destruct H2 as [-> ->]. simpl...
+  - intros. apply NoDup_cons in H as []. assert (Hl:=of_same_length_rest H').
+    apply zip_pair_Permutation_cons_inv_l in H1...
+    destruct H1 as (xs'0&ys'0&xs'1&ys'1&?&?&?&?&?). destruct r.
+    + erewrite split_asgn_list_cons_open. rewrite asgn_xs_with_open. rewrite asgn_ts_with_open.
+      subst.
+      rewrite IH with (lhs':=xs'0 ++ xs'1) (rhs':=ys'0 ++ ys'1)...
+      2:{ apply NoDup_app in H0 as [? []]. apply NoDup_cons in H3 as []. apply NoDup_app.
+          split_and!... intros. apply H1 in H6. set_solver. }
+      repeat erewrite asgn_xs_app. repeat erewrite asgn_ts_app.
+      erewrite split_asgn_list_cons_open. rewrite asgn_xs_with_open. rewrite asgn_ts_with_open...
+      Unshelve. typeclasses eauto.
+    + subst. erewrite asgn_xs_app. erewrite asgn_ts_app.
+      repeat erewrite split_asgn_list_cons_closed. repeat erewrite asgn_xs_with_closed.
+      repeat erewrite asgn_ts_with_closed. rewrite zip_pair_Permutation_app_comm.
+      2:{ apply asgn_of_same_length. }
+      2:{ eapply of_same_length_cons. Unshelve. apply asgn_of_same_length. }
+      simpl. apply zip_pair_Permutation_cons.
+      1:{ apply asgn_of_same_length. }
+      1:{ eapply of_same_length_app. Unshelve. all: apply asgn_of_same_length. }
+      rewrite IH with (lhs':=xs'1 ++ xs'0) (rhs':=ys'1 ++ ys'0)...
+      2:{ apply NoDup_app in H0 as (?&?&?). apply NoDup_cons in H3 as []. apply NoDup_app.
+          split_and!... intros. intros contra. apply H1 in contra. set_solver. }
+      2:{ rewrite zip_pair_Permutation_app_comm... }
+      erewrite asgn_xs_app. erewrite asgn_ts_app...
+      Unshelve. typeclasses eauto.
+Qed.
+
+Local Lemma PAsgnWithOpens_equiv' xs1 rhs1 xs2 rhs2 `{!OfSameLength xs1 rhs1} `{!OfSameLength xs2 rhs2} :
+  NoDup xs1 →
+  NoDup xs2 →
+  asgn_opens (split_asgn_list xs1 rhs1) ≡ₚ asgn_opens (split_asgn_list xs2 rhs2) →
+  (asgn_xs (split_asgn_list xs1 rhs1), asgn_ts (split_asgn_list xs1 rhs1)) ≡ₚₚ
+    (asgn_xs (split_asgn_list xs2 rhs2), asgn_ts (split_asgn_list xs2 rhs2)) →
+  @PAsgnWithOpens M xs1 rhs1 _ ≡ PAsgnWithOpens xs2 rhs2.
+Proof with auto.
+  intros Hnodup1 Hnodup2 Hopens Hclosed A. unfold PAsgnWithOpens.
+  destruct (split_asgn_list xs1 rhs1) eqn:E1. simpl in *.
+  destruct (split_asgn_list xs2 rhs2) eqn:E2. simpl in *. apply wp_proper_prog.
+  rewrite p_varlist_permute.
+  2:{ apply Hopens. }
+  f_equiv. clear A Hopens. intros A. simpl. apply msubst_zip_pair_Permutation.
+  - apply NoDup_fmap.
+    + apply as_var_inj.
+    + eapply submseteq_NoDup; [exact Hnodup1|].
+      replace asgn_xs with (Prog.asgn_xs (split_asgn_list xs1 rhs1)).
+      * apply asgn_xs_submseteq.
+      * rewrite E1. reflexivity.
+  - apply NoDup_fmap.
+    + apply as_var_inj.
+    + eapply submseteq_NoDup; [exact Hnodup2|].
+      replace asgn_xs0 with (Prog.asgn_xs (split_asgn_list xs2 rhs2)).
+      * apply asgn_xs_submseteq.
+      * rewrite E2. reflexivity.
+  - apply zip_pair_Permutation_fmap; try typeclasses eauto...
+Qed.
+
+Lemma PAsgnWithOpens_equiv lhs1 rhs1 lhs2 rhs2 `{!OfSameLength lhs1 rhs1} `{!OfSameLength lhs2 rhs2} :
+  NoDup lhs1 →
+  NoDup lhs2 →
+  (lhs1, rhs1) ≡ₚₚ (lhs2, rhs2) →
+  @PAsgnWithOpens M lhs1 rhs1 _ ≡ PAsgnWithOpens lhs2 rhs2.
+Proof with auto.
+  intros.
+  apply PAsgnWithOpens_equiv'...
+  - apply asgn_opens_Permutation...
+  - apply asgn_xs_ts_Permutation...
+Qed.
+
+Lemma PAsgnWithOpens_wp_equiv (A : final_formula) lhs1 rhs1 lhs2 rhs2 `{!OfSameLength lhs1 rhs1} `{!OfSameLength lhs2 rhs2} :
+  NoDup lhs1 →
+  NoDup lhs2 →
+  (lhs1, rhs1) ≡ₚₚ (lhs2, rhs2) →
+  wp (PAsgnWithOpens lhs1 rhs1) A ≡ wp (PAsgnWithOpens lhs2 rhs2) A.
+Proof with auto.
+  intros. apply PAsgnWithOpens_equiv...
+Qed.
+
+  (* Lemma wp_PAsgnWithOpens (lhs : list final_variable) (rhs : list (@asgn_rhs_term M)) *)
+  (*                         `{!OfSameLength lhs rhs} : *)
+  (*   NoDup lhs → *)
+  (*   ∃ opens xs ts (Hl : OfSameLength xs ts), *)
+  (*     PAsgnWithOpens lhs rhs ≡ PVarList opens (PAsgn xs ts) ∧ *)
+  (*       (∀ x, x ∈ opens ↔ (x, OpenRhsTerm) ∈ (lhs, rhs)) ∧ *)
+  (*       (∀ x t, (x, t) ∈ (xs, ts) ↔ (x, FinalRhsTerm t) ∈ (lhs, rhs)). *)
+  (* Proof with auto. *)
+  (*   intros. *)
+  (*   exists (asgn_opens (split_asgn_list lhs rhs)). *)
+  (*   exists (asgn_xs (split_asgn_list lhs rhs)). *)
+  (*   exists (asgn_ts (split_asgn_list lhs rhs)). *)
+  (*   exists (asgn_of_same_length (split_asgn_list lhs rhs)). *)
+  (*   split_and!. *)
+  (*   - unfold PAsgnWithOpens. destruct (split_asgn_list lhs rhs). simpl. reflexivity. *)
+  (*   - intros. rewrite elem_of_asgn_opens... *)
+  (*     induction_same_length lhs rhs as l r. *)
+  (*     + simpl. rewrite elem_of_nil. rewrite elem_of_zip_pair. set_solver. *)
+  (*     + intros. assert (Hl := of_same_length_rest H'). apply NoDup_cons in H as []. *)
+  (*       destruct (decide (x = l)). *)
+  (*       2:{ ospecialize (IH _ H0). rewrite elem_of_zip_pair_hd_ne... destruct r. *)
+  (*           - erewrite split_asgn_list_cons_open. rewrite asgn_opens_with_open. *)
+  (*             rewrite elem_of_cons. rewrite IH. naive_solver. *)
+  (*           - erewrite split_asgn_list_cons_closed. rewrite asgn_opens_with_closed. *)
+  (*             rewrite IH. reflexivity. } *)
+  (*       subst l. rewrite elem_of_zip_pair_hd... destruct r. *)
+  (*       * erewrite split_asgn_list_cons_open. rewrite asgn_opens_with_open. rewrite elem_of_cons. *)
+
+  (*       } *)
+  (*       } *)
+  (*             set_solver. *)
+  (*           elem_of_zip_pair_ne *)
+  (*           - admit. *)
+  (*           - destruct IH as (i&?). exists (S i). apply elem_of_zip_pair_tl_indexed... } *)
+  (*       subst l. *)
+  (*         destruct r. *)
+  (*           - *)
+  (*       destruct r. *)
+  (*       * exists 0. *)
+  (*   induction_same_length lhs rhs as x r. *)
+  (*   - exists [], [], [], of_same_length_nil. split_and!... *)
+  (*     + intros. set_solver. *)
+  (*     + intros. apply elem_of_zip_pair in H1. set_solver. *)
+  (*   - intros. assert (Hl:=of_same_length_rest H'). *)
+  (*     apply NoDup_cons in H as []. specialize (IH Hl H0). *)
+  (*     destruct IH as (opens&xs&ts&?&?&?&?). destruct r eqn:E. *)
+  (*     + exists (opens ++ [x]), xs, ts, x0. split_and!... *)
+  (*       * unfold PAsgnWithOpens. unfold PAsgnWithOpens in H1. *)
+  (*         erewrite split_asgn_list_cons_open. unfold asgn_args_with_open. *)
+  (*         destruct (split_asgn_list lhs rhs) eqn:E'. *)
+  (*         simpl. rewrite H1. rewrite p_varlist_app. simpl... *)
+  (*       * intros. set_unfold in H4. destruct_or! H4. *)
+  (*         -- apply H2 in H4 as (i&?). exists (S i). rewrite elem_of_zip_pair_tl_indexed... *)
+  (*         -- subst. exists 0. rewrite elem_of_zip_pair_hd_indexed. split... *)
+  (*       * intros. apply H3 in H4. destruct H4 as (i&?). *)
+  (*         apply elem_of_zip_pair_indexed in H4. simpl in H4. exists (S i). *)
+  (*         rewrite elem_of_zip_pair_tl_indexed... *)
+  (*     + exists opens, (xs ++ [x]), (ts ++ [t]), _. split_and!... *)
+  (*       * unfold PAsgnWithOpens. unfold PAsgnWithOpens in H1. *)
+  (*         erewrite split_asgn_list_cons_closed. unfold asgn_args_with_closed. *)
+  (*         destruct (split_asgn_list lhs rhs) eqn:E'. *)
+  (*         simpl. intros A. specialize (H1 A). *)
+  (*         rewrite H1. rewrite p_varlist_app. simpl... *)
+  (*       * intros. set_unfold in H4. destruct_or! H4. *)
+  (*         -- apply H2 in H4 as (i&?). exists (S i). rewrite elem_of_zip_pair_tl_indexed... *)
+  (*         -- subst. exists 0. rewrite elem_of_zip_pair_hd_indexed. split... *)
+  (*       * intros. apply H3 in H4. destruct H4 as (i&?). *)
+  (*         apply elem_of_zip_pair_indexed in H4. simpl in H4. exists (S i). *)
+  (*         rewrite elem_of_zip_pair_tl_indexed... *)
+  (*     + *)
+  (*         destruct H4 as (?&?). *)
+  (*         -- *)
+  (*     `{!OfSameLength xs0 rhs0} *)
+  (*     `{!OfSameLength xs1 rhs1} *)
+  (*     `{!OfSameLength xs2 rhs2} *)
+  (*     {Hl1 Hl2} : *)
+  (*   @PAsgnWithOpens M (xs0 ++ [x1] ++ xs1 ++ [x2] ++ xs2) *)
+  (*     (rhs0 ++ [r1] ++ rhs1 ++ [r2] ++ rhs2) Hl1 ≡ *)
+  (*   @PAsgnWithOpens M (xs0 ++ [x2] ++ xs1 ++ [x1] ++ xs2) *)
+  (*     (rhs0 ++ [r2] ++ rhs1 ++ [r1] ++ rhs2) Hl2. *)
+
+  (* Lemma msubst_comm xs0 (rhs0 : list asgn_rhs_term) x1 r1 xs1 rhs1 x2 r2 xs2 rhs2 *)
+  (*     `{!OfSameLength xs0 rhs0} *)
+  (*     `{!OfSameLength xs1 rhs1} *)
+  (*     `{!OfSameLength xs2 rhs2} *)
+  (*     {Hl1 Hl2} : *)
+  (*   @PAsgnWithOpens M (xs0 ++ [x1] ++ xs1 ++ [x2] ++ xs2) *)
+  (*     (rhs0 ++ [r1] ++ rhs1 ++ [r2] ++ rhs2) Hl1 ≡ *)
+  (*   @PAsgnWithOpens M (xs0 ++ [x2] ++ xs1 ++ [x1] ++ xs2) *)
+  (*     (rhs0 ++ [r2] ++ rhs1 ++ [r1] ++ rhs2) Hl2. *)
+  (* Proof with auto. *)
+  (*   intros A. unfold PAsgnWithOpens. split_asgn_list *)
+  (*   intros A. *)
+  (*   generalize dependent rhs1. generalize dependent rhs0. *)
+  (*   generalize dependent xs1. generalize dependent xs0. *)
+  (*   induction_same_length xs2 rhs2 as x2' r2'. *)
+  (*   - simpl. induction_same_length xs1 rhs1 as x1' r1'. *)
+  (*     + simpl. admit. *)
+  (*     + intros. simpl. erewrite *)
+  (*   - intros. *)
+  (*   generalize dependent rhs2. *)
+  (*   generalize dependent rhs2. *)
+  (*   generalize dependent rhs2. *)
+  (*   generalize dependent rhs2. *)
+  (*   generalize dependent rhs2. *)
+
+  (* (*                   Hl1 *) *)
+  (* (*   <{ *xs0, x1, *xs1, x2, *xs2 := *rhs0, *$([r1]), *rhs1, *$([r2]), *rhs2 }> ≡ *) *)
+  (* (*   <{ *xs0, x2, *xs1, x1, *xs2 := *rhs0, *$([r2]), *rhs1, *$([r1]), *rhs2 }>. *) *)
+  (* (*   msubst A (@to_var_term_map _ (xs0 ++ [x1] ++ xs1 ++ [x2] ++ xs2) *) *)
+  (* (*               (rhs0 ++ [t1] ++ rhs1 ++ [t2] ++ rhs2) Hl1) ≡ *) *)
+  (* (*   msubst A (@to_var_term_map _ (xs0 ++ [x2] ++ xs1 ++ [x1] ++ xs2) *) *)
+  (* (*               (rhs0 ++ [t2] ++ rhs1 ++ [t1] ++ rhs2) Hl2). *) *)
+  (* (* Proof with auto. *) *)
+
+  (* (* Lemma asgn_comm' x r xs1 xs2 (rhs1 rhs2 : list (@asgn_rhs_term M)) *) *)
+  (* (*     `{!OfSameLength xs1 rhs1} *) *)
+  (* (*     `{!OfSameLength xs2 rhs2} : *) *)
+  (* (*   <{ x, *xs1, *xs2 := *$([r]), *rhs1, *rhs2 }> ≡ *) *)
+  (* (*   <{ *xs1, x, *xs2 := *rhs1, *$([r]), *rhs2 }>. *) *)
+  (* (* Proof with auto. *) *)
+  (* (*   intros A. *) *)
+  (* (*   generalize dependent r. generalize dependent x. *) *)
+  (* (*   generalize dependent rhs1. generalize dependent xs1. *) *)
+  (* (*   induction_same_length xs2 rhs2 as x2 r2... *) *)
+  (* (*   - simpl. induction_same_length xs1 rhs1 as x1 r1... simpl. *) *)
+  (* (*     + simpl... *) *)
+  (* (*   intros *) *)
+  (* (*   - simpl... *) *)
+  (* (*   - intros. *) *)
+  (* (*   generalize dependent r. generalize dependent x. *) *)
+  (* (*   induction_same_length xs rhs as x' r'... intros. simpl. *) *)
+  (* (* Lemma asgn_comm' x r xs (rhs : list (@asgn_rhs_term M)) *) *)
+  (* (*     `{!OfSameLength xs rhs} *) *)
+  (* (*     `{!OfSameLength (x :: xs) (r :: rhs)} : *) *)
+  (* (*   <{ x, *xs := *$([r]), *rhs }> ≡ *) *)
+  (* (*   <{ *xs, x := *rhs, *$([r]) }>. *) *)
+  (* (* Proof with auto. *) *)
+  (* (*   intros A. generalize dependent r. generalize dependent x. *) *)
+  (* (*   induction_same_length xs rhs as x' r'... intros. *) *)
+  (* (*   intros *) *)
+  (* (*   - simpl... *) *)
+  (* (*   - intros. *) *)
+  (* (*   generalize dependent r. generalize dependent x. *) *)
+  (* (*   induction_same_length xs rhs as x' r'... intros. simpl. *) *)
+  (* (* Lemma asgn_comm' x r xs (rhs : list (@asgn_rhs_term M)) *) *)
+  (* (*     `{!OfSameLength xs rhs} *) *)
+  (* (*     `{!OfSameLength (xs ++ [x]) (rhs ++ [r])} : *) *)
+  (* (*   (* x ∉ xs2 → *) *) *)
+  (* (*   (* NoDup xs2 → *) *) *)
+  (* (*   <{ *xs, x := *rhs, *$([r]) }> ≡ *) *)
+  (* (*   <{ x, *xs := *$([r]), *rhs }>. *) *)
+  (* (* Proof with auto. *) *)
+  (* (*   intros A. generalize dependent r. generalize dependent x. *) *)
+  (* (*   induction_same_length xs rhs as x1 r1... intros. *) *)
+  (* (*   erewrite (rewrite_of_same_length *) *)
+  (* (*               _ (x1 :: (xs ++ [x])) *) *)
+  (* (*               _ (r1 :: (rhs ++ [r])))... *) *)
+  (* (*   destruct r1, r. *) *)
+  (* (*   - simpl. repeat erewrite PAsgnWithOpens_cons_open. simpl. admit. *) *)
+  (* (*   - repeat erewrite PAsgnWithOpens_cons_open. simpl. *) *)
+  (* (*     unfold PAsgnWithOpens. *) *)
+  (* (*     erewrite split_asgn_list_cons_closed. erewrite split_asgn_list_cons_closed. *) *)
+  (* (*     erewrite split_asgn_list_cons_open. *) *)
+  (* (*     unfold asgn_args_with_closed. unfold asgn_args_with_open. *) *)
+  (* (*     destruct (split_asgn_list (xs1 ++ xs2) (rhs1 ++ rhs2)) eqn:E. *) *)
+  (* (*     simpl. repeat f_equiv. *) *)
+  (* (*   + repeat erewrite PAsgnWithOpens_cons_open. simpl. *) *)
+  (* (*     unfold PAsgnWithOpens. *) *)
+  (* (*     erewrite split_asgn_list_cons_closed. erewrite split_asgn_list_cons_closed. *) *)
+  (* (*     erewrite split_asgn_list_cons_open. *) *)
+  (* (*     unfold asgn_args_with_closed. unfold asgn_args_with_open. *) *)
+  (* (*     destruct (split_asgn_list (xs1 ++ xs2) (rhs1 ++ rhs2)) eqn:E. *) *)
+  (* (*     simpl. repeat f_equiv. *) *)
+  (* (*   + simpl. unfold PAsgnWithOpens. *) *)
+  (* (*     erewrite split_asgn_list_cons_closed. erewrite split_asgn_list_cons_closed. *) *)
+  (* (*     erewrite split_asgn_list_cons_closed. erewrite split_asgn_list_cons_closed. *) *)
+  (* (*     unfold asgn_args_with_closed. *) *)
+  (* (*     destruct (split_asgn_list (xs1 ++ xs2) (rhs1 ++ rhs2)) eqn:E. *) *)
+  (* (*     simpl. clear E. induction asgn_opens; simpl; [| rewrite IHasgn_opens; auto]. *) *)
+  (* (*     erewrite (rewrite_of_same_length *) *)
+  (* (*                 _ ([] ++ [as_var x] ++ [as_var x2] ++ (list_fmap final_variable variable as_var asgn_xs)) *) *)
+  (* (*                 _ ([] ++ [as_term t] ++ [as_term t0] ++ list_fmap final_term term as_term asgn_ts))... *) *)
+  (* (*     rewrite (msubst_comm_consecutive A [] [] (as_var x) (as_term t) (as_var x2) (as_term t0))... *) *)
+  (* (*     1-2: typeclasses eauto. *) *)
+  (* (*     Set Printing Coercions. intros contra. apply as_var_inj in contra. subst. done. *) *)
+
+  (* (*   generalize dependent rhs2. generalize dependent xs2. *) *)
+  (* (*   induction_same_length xs1 rhs1 as x1 r1. *) *)
+  (* (*   - simpl. intros A. simpl. erewrite PAsgnWithOpens_app_nil_r... *) *)
+  (* (*   - intros. intros A. simpl. *) *)
+  (* (*   <{ x, *xs := *[r], *rhs }>. *) *)
+  (* (* Proof with auto. *) *)
+  (* (*   generalize dependent r. generalize dependent x. *) *)
+  (* (*   induction_same_length xs rhs as x' r'... intros. simpl. *) *)
+  (* Lemma asgn_comm x r xs1 xs2 (rhs1 rhs2 : list (@asgn_rhs_term M)) *)
+  (*     `{!OfSameLength xs1 rhs1} *)
+  (*     `{!OfSameLength xs2 rhs2} *)
+  (*     `{!OfSameLength (xs1 ++ [x]) (rhs1 ++ [r])} *)
+  (*     `{!OfSameLength (xs1 ++ [x] ++ xs2) (rhs1 ++ [r] ++ rhs2)} : *)
+  (*   x ∉ xs2 → *)
+  (*   NoDup xs2 → *)
+  (*   <{ *xs1, x, *xs2 := *rhs1, *[r], *rhs2 }> ≡ *)
+  (*   <{ x, *xs1, *xs2 := *[r], *rhs1, *rhs2 }>. *)
+  (* Proof with auto. *)
+  (*   generalize dependent rhs2. generalize dependent xs2. *)
+  (*   generalize dependent r. generalize dependent x. *)
+  (*   induction_same_length xs1 rhs1 as x1 r1. *)
+  (*   - simpl. f_equiv. apply OfSameLength_pi. *)
+  (*   - intros. *)
+
+  (*     destruct r, r1. *)
+  (*     + simpl. admit. *)
+  (*     + repeat erewrite PAsgnWithOpens_cons_open. simpl. *)
+  (*       unfold PAsgnWithOpens. *)
+  (*       erewrite split_asgn_list_cons_closed. erewrite split_asgn_list_cons_closed. *)
+  (*       erewrite split_asgn_list_cons_open. *)
+  (*       unfold asgn_args_with_closed. unfold asgn_args_with_open. *)
+  (*       destruct (split_asgn_list (xs1 ++ xs2) (rhs1 ++ rhs2)) eqn:E. *)
+  (*       simpl. repeat f_equiv. *)
+
+  (*     + repeat erewrite PAsgnWithOpens_cons_open. simpl. *)
+  (*       unfold PAsgnWithOpens. *)
+  (*       erewrite split_asgn_list_cons_closed. erewrite split_asgn_list_cons_closed. *)
+  (*       erewrite split_asgn_list_cons_open. *)
+  (*       unfold asgn_args_with_closed. unfold asgn_args_with_open. *)
+  (*       destruct (split_asgn_list (xs1 ++ xs2) (rhs1 ++ rhs2)) eqn:E. *)
+  (*       simpl. repeat f_equiv. *)
+  (*     +  *)
+
+  (*     + opose proof (IH _ _ _) as []. intros A.  *)
+  (*   simpl. intros Hdisj Hnodup. generalize dependent rhs1. generalize dependent xs1. *)
+  (*   generalize dependent r. generalize dependent x. induction_same_length xs2 rhs2 as x2 r2. *)
+  (*   - induction_same_length xs1 rhs1 as x1 r1... intros. simpl. split. *)
+  (*      s *)
+  (*   - intros. assert (Hl := of_same_length_rest H'). *)
+  (*     erewrite (rewrite_of_same_length _ *)
+  (*                 ((xs1 ++ [x]) ++ (x2 :: xs2)) _ ((rhs1 ++ [r]) ++ (r2 :: rhs2))). *)
+  (*     2-3: rewrite cons_middle; rewrite app_assoc... *)
+  (*     apply NoDup_cons in Hnodup as []. apply not_elem_of_cons in Hdisj as []. rewrite IH... *)
+  (*     erewrite (rewrite_of_same_length _ *)
+  (*                 ((x2 :: xs1) ++ (x :: xs2)) _ ((r2 :: rhs1) ++ (r :: rhs2))). *)
+  (*     2-3: rewrite <- app_assoc; rewrite cons_middle; rewrite app_comm_cons... *)
+  (*     rewrite IH... *)
+  (*     erewrite (rewrite_of_same_length *)
+  (*                 (x :: (xs1 ++ x2 :: xs2)) ((x :: xs1) ++ (x2 :: xs2)) *)
+  (*                 _ ((r :: rhs1) ++ (r2 :: rhs2))). *)
+  (*     2-3: rewrite app_comm_cons... *)
+  (*     rewrite IH... simpl. clear IH. *)
+  (*     Unshelve. 2-7: typeclasses eauto. *)
+  (*     destruct r, r2. *)
+  (*     + repeat erewrite PAsgnWithOpens_cons_open. simpl. rewrite f_forall_comm... *)
+  (*     + repeat erewrite PAsgnWithOpens_cons_open. simpl. *)
+  (*       unfold PAsgnWithOpens. *)
+  (*       erewrite split_asgn_list_cons_closed. erewrite split_asgn_list_cons_closed. *)
+  (*       erewrite split_asgn_list_cons_open. *)
+  (*       unfold asgn_args_with_closed. unfold asgn_args_with_open. *)
+  (*       destruct (split_asgn_list (xs1 ++ xs2) (rhs1 ++ rhs2)) eqn:E. *)
+  (*       simpl. repeat f_equiv. *)
+  (*     + repeat erewrite PAsgnWithOpens_cons_open. simpl. *)
+  (*       unfold PAsgnWithOpens. *)
+  (*       erewrite split_asgn_list_cons_closed. erewrite split_asgn_list_cons_closed. *)
+  (*       erewrite split_asgn_list_cons_open. *)
+  (*       unfold asgn_args_with_closed. unfold asgn_args_with_open. *)
+  (*       destruct (split_asgn_list (xs1 ++ xs2) (rhs1 ++ rhs2)) eqn:E. *)
+  (*       simpl. repeat f_equiv. *)
+  (*     + simpl. unfold PAsgnWithOpens. *)
+  (*       erewrite split_asgn_list_cons_closed. erewrite split_asgn_list_cons_closed. *)
+  (*       erewrite split_asgn_list_cons_closed. erewrite split_asgn_list_cons_closed. *)
+  (*       unfold asgn_args_with_closed. *)
+  (*       destruct (split_asgn_list (xs1 ++ xs2) (rhs1 ++ rhs2)) eqn:E. *)
+  (*       simpl. clear E. induction asgn_opens; simpl; [| rewrite IHasgn_opens; auto]. *)
+  (*       erewrite (rewrite_of_same_length *)
+  (*                   _ ([] ++ [as_var x] ++ [as_var x2] ++ (list_fmap final_variable variable as_var asgn_xs)) *)
+  (*                   _ ([] ++ [as_term t] ++ [as_term t0] ++ list_fmap final_term term as_term asgn_ts))... *)
+  (*       rewrite (msubst_comm_consecutive A [] [] (as_var x) (as_term t) (as_var x2) (as_term t0))... *)
+  (*       1-2: typeclasses eauto. *)
+  (*       Set Printing Coercions. intros contra. apply as_var_inj in contra. subst. done. *)
+
+  (* Lemma asgn_comm x r xs1 xs2 (rhs1 rhs2 : list (@asgn_rhs_term M)) *)
+  (*     `{!OfSameLength xs1 rhs1} *)
+  (*     `{!OfSameLength xs2 rhs2} *)
+  (*     `{!OfSameLength (xs1 ++ [x] ++ xs2) (rhs1 ++ [r] ++ rhs2)} : *)
+  (*   x ∉ xs2 → *)
+  (*   NoDup xs2 → *)
+  (*   <{ *xs1, x, *xs2 := *rhs1, *[r], *rhs2 }> ≡ *)
+  (*   <{ x, *xs1, *xs2 := *[r], *rhs1, *rhs2 }>. *)
+  (* Proof with auto. *)
+  (*   simpl. intros Hdisj Hnodup A. generalize dependent rhs1. generalize dependent xs1. *)
+  (*   generalize dependent r. generalize dependent x. induction_same_length xs2 rhs2 as x2 r2. *)
+  (*   (* - unfold PAsgnWithOpens.  *) *)
+
+  (*   - *)
+
+  (*     generalize dependent r. generalize dependent x. *)
+  (*     induction_same_length xs1 rhs1 as x1 r1... intros. simpl. destruct r1, r. *)
+  (*     + admit. *)
+  (*     + admit. *)
+  (*     + unfold PAsgnWithOpens. *)
+  (*       erewrite split_asgn_list_cons_open. *)
+  (*       repeat erewrite split_asgn_list_cons_closed. *)
+  (*       assert (Hl:=of_same_length_rest H'). *)
+  (*       destruct (split_asgn_list xs1 rhs1) eqn:E. *)
+
+
+
+  (*   - intros. assert (Hl := of_same_length_rest H'). *)
+  (*     erewrite (rewrite_of_same_length _ *)
+  (*                 ((xs1 ++ [x]) ++ (x2 :: xs2)) _ ((rhs1 ++ [r]) ++ (r2 :: rhs2))). *)
+  (*     2-3: rewrite cons_middle; rewrite app_assoc... *)
+  (*     apply NoDup_cons in Hnodup as []. apply not_elem_of_cons in Hdisj as []. rewrite IH... *)
+  (*     erewrite (rewrite_of_same_length _ *)
+  (*                 ((x2 :: xs1) ++ (x :: xs2)) _ ((r2 :: rhs1) ++ (r :: rhs2))). *)
+  (*     2-3: rewrite <- app_assoc; rewrite cons_middle; rewrite app_comm_cons... *)
+  (*     rewrite IH... *)
+  (*     erewrite (rewrite_of_same_length *)
+  (*                 (x :: (xs1 ++ x2 :: xs2)) ((x :: xs1) ++ (x2 :: xs2)) *)
+  (*                 _ ((r :: rhs1) ++ (r2 :: rhs2))). *)
+  (*     2-3: rewrite app_comm_cons... *)
+  (*     rewrite IH... simpl. clear IH. *)
+  (*     Unshelve. 2-7: typeclasses eauto. *)
+  (*     destruct r, r2. *)
+  (*     + repeat erewrite PAsgnWithOpens_cons_open. simpl. rewrite f_forall_comm... *)
+  (*     + repeat erewrite PAsgnWithOpens_cons_open. simpl. *)
+  (*       unfold PAsgnWithOpens. *)
+  (*       erewrite split_asgn_list_cons_closed. erewrite split_asgn_list_cons_closed. *)
+  (*       erewrite split_asgn_list_cons_open. *)
+  (*       unfold asgn_args_with_closed. unfold asgn_args_with_open. *)
+  (*       destruct (split_asgn_list (xs1 ++ xs2) (rhs1 ++ rhs2)) eqn:E. *)
+  (*       simpl. repeat f_equiv. *)
+  (*     + repeat erewrite PAsgnWithOpens_cons_open. simpl. *)
+  (*       unfold PAsgnWithOpens. *)
+  (*       erewrite split_asgn_list_cons_closed. erewrite split_asgn_list_cons_closed. *)
+  (*       erewrite split_asgn_list_cons_open. *)
+  (*       unfold asgn_args_with_closed. unfold asgn_args_with_open. *)
+  (*       destruct (split_asgn_list (xs1 ++ xs2) (rhs1 ++ rhs2)) eqn:E. *)
+  (*       simpl. repeat f_equiv. *)
+  (*     + simpl. unfold PAsgnWithOpens. *)
+  (*       erewrite split_asgn_list_cons_closed. erewrite split_asgn_list_cons_closed. *)
+  (*       erewrite split_asgn_list_cons_closed. erewrite split_asgn_list_cons_closed. *)
+  (*       unfold asgn_args_with_closed. *)
+  (*       destruct (split_asgn_list (xs1 ++ xs2) (rhs1 ++ rhs2)) eqn:E. *)
+  (*       simpl. clear E. induction asgn_opens; simpl; [| rewrite IHasgn_opens; auto]. *)
+  (*       erewrite (rewrite_of_same_length *)
+  (*                   _ ([] ++ [as_var x] ++ [as_var x2] ++ (list_fmap final_variable variable as_var asgn_xs)) *)
+  (*                   _ ([] ++ [as_term t] ++ [as_term t0] ++ list_fmap final_term term as_term asgn_ts))... *)
+  (*       rewrite (msubst_comm_consecutive A [] [] (as_var x) (as_term t) (as_var x2) (as_term t0))... *)
+  (*       1-2: typeclasses eauto. *)
+  (*       Set Printing Coercions. intros contra. apply as_var_inj in contra. subst. done. *)
+
+
+  (* Lemma asgn_comm xs1 xs2 (rhs1 rhs2 : list (@asgn_rhs_term M)) *)
+  (*   `{!OfSameLength xs1 rhs1} *)
+  (*   `{!OfSameLength xs2 rhs2} : *)
+  (*   <{ *xs1, *xs2 := *rhs1, *rhs2 }> ⊑ *)
+  (*   <{ *xs2, *xs1 := *rhs2, *rhs1 }>. *)
+  (* Proof. *)
+  (*   intros A. generalize dependent rhs2. generalize dependent xs2. *)
+  (*   induction_same_length xs1 rhs1 as x1 r1; intros. *)
+  (*   - simpl. admit. *)
+  (*   - destruct r1. *)
+  (*     + simpl. *)
+  (*       erewrite PAsgnWithOpens_cons_open. simpl. rewrite IH. *)
+  (*       ospecialize (IH _ (xs2 ++ [x1]) (rhs2 ++ [OpenRhsTerm]) _). *)
+  (*       simpl in IH. *)
+  (*       rewrite <- IH. *)
+  (*       opose proof (@PAsgnWithOpens_cons_open _ x1 (xs1 ++ xs2) (rhs1 ++ rhs2) _). *)
+  (*       rewrite H. *)
+
+  Lemma r_open_assignment x (t : final_term) xs0 xs1 (rhs0 rhs1 : list (@asgn_rhs_term M))
+    `{!OfSameLength xs0 rhs0}
+    `{!OfSameLength xs1 rhs1} :
+    x ∉ xs0 →
+    x ∉ xs1 →
+    NoDup xs0 →
+    NoDup xs1 →
+    xs0 ## xs1 →
+    <{ *xs0, x, *xs1 := *rhs0, ?, *rhs1 }> ⊑
+    <{ *xs0, x, *xs1 := *rhs0, t, *rhs1 }>.
+  Proof with auto.
+    intros. intros A.
+    rewrite PAsgnWithOpens_wp_equiv with (lhs2:=x :: xs0 ++ xs1)
+                                                    (rhs2:=OpenRhsTerm :: rhs0 ++ rhs1)...
+    2:{ apply NoDup_app. split_and!; [auto | set_solver |]. simpl. apply NoDup_cons.
+        split... }
+    3:{ simpl. rewrite zip_pair_Permutation_app_comm...
+        2: typeclasses eauto. simpl. apply zip_pair_Permutation_cons...
+        1-2: typeclasses eauto. rewrite zip_pair_Permutation_app_comm... }
+    2:{ apply NoDup_cons. rewrite NoDup_app. split_and!... set_solver. }
+    rewrite PAsgnWithOpens_wp_equiv with (lhs1:=xs0 ++ [x] ++ xs1) (lhs2:=x :: xs0 ++ xs1)
+                                                    (rhs2:=FinalRhsTerm t :: rhs0 ++ rhs1)...
+    2:{ apply NoDup_app. split_and!; [auto | set_solver |]. simpl. apply NoDup_cons.
+        split... }
+    3:{ simpl. rewrite zip_pair_Permutation_app_comm...
+        2: typeclasses eauto. simpl. rewrite as_final_term_as_term.
+        apply zip_pair_Permutation_cons...
+        1-2: typeclasses eauto. rewrite zip_pair_Permutation_app_comm... }
+    2:{ apply NoDup_cons. rewrite NoDup_app. split_and!... set_solver. }
+    unfold PAsgnWithOpens.
+    destruct (split_asgn_list (x :: xs0 ++ xs1) (OpenRhsTerm :: rhs0 ++ rhs1)) eqn:E1.
+    destruct (split_asgn_list (x :: xs0 ++ xs1) (FinalRhsTerm t :: rhs0 ++ rhs1)) eqn:E2.
+
+    assert (OfSameLength (xs0 ++ xs1) (rhs0 ++ rhs1)).
+    { unfold OfSameLength in *. repeat rewrite length_app. lia. }
+    rewrite split_asgn_list_cons_open with (OfSameLength0:=H4) in E1.
+    rewrite split_asgn_list_cons_closed with (Hl1:=H4) in E2.
+    unfold asgn_args_with_open in E1. unfold asgn_args_with_closed in E2.
+    simpl in E1, E2.
+    destruct (split_asgn_list (xs0 ++ xs1) (rhs0 ++ rhs1)).
+    inversion E1. inversion E2. clear E1 E2. subst. simpl.
+    repeat rewrite wp_varlist. simpl. rewrite f_forall_elim with (t:=t).
+    rewrite E2 in E1.
+    inversion E. simpl.
+    erewrite split_asgn_list_cons_open.
+    destr
+    unfold asgn_args_with_open. simpl.
+    unfold asgn
+    simpl.
+        - typeclasses eauto.
+        split... }
+        - intros. set_solver.
+        - apply NoDup_app.
+    intros A. induction_same_length xs ts as x t.
+    - simpl. apply fequiv_congr. repeat f_equiv. apply OfSameLength_pi.
+    - simpl.
+    - simpl.
+    simpl.
+
 
   (* Law 4.1 *)
   Lemma r_alternation w pre post gs `{!FormulaFinal pre} :
